Experiments with global proof. Assumptions about Linker

stanfrontend/Scompiler.v
@@ -17,6 +17,8 @@ Require Import Sbackend.
 Require Import Coqlib.
 Require Import Linking. 
 
+Require Import Sbackendproof.
+
 Open Scope string_scope.
 Local Open Scope linking_scope.
 
@@ -34,7 +36,54 @@ Definition transf_stan_program(p: StanE.program): res Clight.program :=
   @@ print (print_CStan 2)
   @@@ time "Target" Target.transf_program
   @@ print (print_CStan 3)
+  @@@ time "Backend" backend. 
+
+
+Definition ProbCompCert's_passes :=
+  mkpass Sbackendproof.match_prog
+  ::: pass_nil _.
+
+Definition match_prog_test: CStan.program -> Clight.program -> Prop :=
+  pass_match (compose_passes ProbCompCert's_passes).
+
+Definition transf_cstan_program(p: CStan.program): res Clight.program :=
+  OK p
   @@@ time "Backend" backend.
+
+Theorem transf_cstan_program_match:
+  forall p tp,
+  transf_cstan_program p = OK tp ->
+  match_prog_test p tp.
+Proof.
+  intros p tp T.
+  unfold transf_cstan_program, time in T. simpl in T. 
+  destruct (Sbackend.backend p) as [p1|e] eqn:P2; simpl in T; try discriminate.
+  unfold match_prog_test; simpl.
+  exists p1; split. eapply Sbackendproof.transf_program_match; eauto. 
+  inversion T.  
+  reflexivity.
+Qed. 
+
+Lemma transf_cstan_program_correct:
+  forall p tp,
+  match_prog_test p tp ->
+  transf_cstan_program p = OK tp ->
+  forward_simulation (CStanSemanticsBackend.semantics p) (Clight.semantics1 tp).
+Proof.
+  intros p tp M. unfold match_prog_test, pass_match in M; simpl in M.
+  Ltac DestructM_test :=
+    match goal with
+      [ H: exists p, _ /\ _ |- _ ] =>
+        let p := fresh "p" in let M := fresh "M" in let MM := fresh "MM" in
+        destruct H as (p & M & MM); clear H
+    end.
+  repeat DestructM_test. subst tp.
+
+  intros.
+  eapply compose_forward_simulations.
+    eapply Sbackendproof.transf_program_correct; eassumption.  
+  eapply forward_simulation_identity; eauto.
+Qed.  
 
 Theorem transf_stan_program_correct:
   forall p tp,
